complete proof

src/logic/FancyUpdate.v
@@ -10,6 +10,8 @@ Section INTERPRETATION.
     ; prop : Var -> iProp
     }.
 
+  Definition interpRA `{Interp} : URA.t := (Auth.t (positive ==> URA.agree Var)%ra).
+
 End INTERPRETATION.
 
 Section PCM_OWN.
@@ -18,7 +20,7 @@ Section PCM_OWN.
 
   Definition OwnE `{@GRA.inG CoPset.t Σ} (E : coPset) := OwnM (Some E).
   Definition OwnD `{@GRA.inG Gset.t Σ} (D : gset positive) := OwnM (Some D).
-  Definition inv `{Interp} `{@GRA.inG (Auth.t (positive ==> URA.agree Var)%ra) Σ}
+  Definition inv `{Interp} `{@GRA.inG interpRA Σ}
     (i : positive) (x : Var) :=
     OwnM (Auth.white (@maps_to_res positive (URA.agree Var) i (Some (Some x)))).
 
@@ -44,7 +46,16 @@ Section PCM_OWN.
 
   Global Instance inv_persistent `{Interp} `{@GRA.inG (Auth.t (positive ==> URA.agree Var)%ra) Σ}
     i p : Persistent (inv i p).
-  Admitted.
+  Proof.
+    unfold inv. remember (Auth.white
+                            (@maps_to_res
+                               positive
+                               (URA.agree Var)
+                               i (Some (Some p)))) as r.
+    unfold Persistent. iIntros "H".
+    iPoseProof (@OwnM_persistently _ _ H0 _ with "H") as "#HP".
+    iModIntro. replace r with (URA.core r) at 2 by (subst; ss). iApply "HP".
+  Qed.
 
 End PCM_OWN.
 
@@ -54,7 +65,7 @@ Section WORLD_SATISFACTION.
   Context `{@Interp Σ}.
   Context `{@GRA.inG CoPset.t Σ}.
   Context `{@GRA.inG Gset.t Σ}.
-  Context `{@GRA.inG (Auth.t (positive ==> URA.agree Var)%ra) Σ}.
+  Context `{@GRA.inG interpRA Σ}.
 
   Definition inv_auth (I : gmap positive Var) :=
     OwnM (@Auth.black
@@ -66,22 +77,108 @@ Section WORLD_SATISFACTION.
 
   Definition wsat : iProp := (∃ I, inv_auth I ∗ inv_satall I)%I.
 
+  Lemma alloc_name (X : gset positive) :
+    ⊢ |==> ∃ i, OwnD {[i]} ∧ ⌜i ∉ X⌝.
+  Proof.
+    assert (@URA.updatable_set Gset.t (Some ∅) (fun r => exists i, r = Some {[i]} /\ i ∉ X)) as UPD.
+    { clear. ii. apply URA.wf_split in WF; des. destruct ctx as [D|].
+      - assert (exists i, i ∉ D /\ i ∉ X) as [i [iD iI]].
+        { exists (fresh (D ∪ X)). pose proof (is_fresh (D ∪ X)). set_solver. }
+        exists (Some {[i]}). split.
+        + exists i. ss.
+        + unfold URA.wf, URA.add. unseal "ra". ss. des_ifs; set_solver.
+      - rr in WF0. unseal "ra". ss.
+    }
+    iPoseProof (@OwnM_unit _ _ H1) as "-# H".
+    iMod (OwnM_Upd_set UPD with "H") as "[% [% DIS]]".
+    iModIntro. des. subst. iExists i. eauto.
+  Qed.
+
   Lemma wsat_inv_alloc p :
     wsat ∗ prop p ⊢ |==> ∃ i, inv i p ∗ wsat.
-  Admitted.
+  Proof.
+    iIntros "[[% [AUTH SAT]] P]".
+    unfold inv_auth, inv_satall.
+    iMod (alloc_name (dom I)) as "[% [D %iI]]".
+    pose (<[i:=p]> I) as I'.
+
+    assert (URA.updatable
+              (@Auth.black (positive ==> URA.agree Var)%ra (fun i => Some <$> (I !! i)))
+              (@Auth.black
+                 (positive ==> URA.agree Var)%ra
+                 (fun i => Some <$> (I' !! i))
+                 ⋅
+                 (@Auth.white
+                    (positive ==> URA.agree Var)%ra
+                    (@maps_to_res _ (URA.agree Var) i (Some (Some p)))))).
+    { apply Auth.auth_alloc. ii. des. rewrite URA.unit_idl in FRAME. subst. split.
+      { rr; unseal "ra". ss. intro. rr; unseal "ra". destruct (I' !! k); ss. }
+      rr. subst I'.
+      unfold URA.add. unseal "ra". ss.
+      extensionalities j. unfold maps_to_res. des_ifs.
+      - rewrite lookup_insert. rewrite not_elem_of_dom_1; ss. 
+        unfold URA.add. unseal "ra". ss.
+      - rewrite URA.unit_idl. rewrite lookup_insert_ne; eauto.
+    }
+    iMod (OwnM_Upd H3 with "AUTH") as "[AUTH NEW]". iModIntro.
+
+    iExists i. iFrame. unfold wsat. iExists I'. iFrame.
+    unfold inv_satall. subst I'.
+    iApply big_sepM_insert. { apply not_elem_of_dom_1; ss. }
+    iSplitL "P D"; ss. iLeft. iFrame.
+  Qed.
 
   Lemma wsat_inv_open i p :
     inv i p ∗ wsat ∗ OwnE {[i]} ⊢ |==> prop p ∗ wsat ∗ OwnD {[i]}.
   Proof.
-    iIntros "(I & [% [AUTH SAT]] & EN)".
+    iIntros "(I & [% [AUTH SAT]] & EN)". iModIntro.
     unfold inv, inv_auth, inv_satall.
-    Search Auth.white.
-    Search OwnM.
-  Admitted.
+    iCombine "AUTH I" as "AUTH".
+    iPoseProof (OwnM_valid with "AUTH") as "%WF".
+    assert (Hip : I !! i = Some p).
+    { apply Auth.auth_included in WF. rename WF into EXTENDS.
+      apply pw_extends in EXTENDS. specialize (EXTENDS i).
+      unfold maps_to_res in EXTENDS. des_ifs. clear e.
+      rr in EXTENDS. des. unfold URA.add in EXTENDS; unseal "ra".
+      destruct (I !! i) eqn: E.
+      - destruct ctx; ss; des_ifs.
+      - destruct ctx; ss; des_ifs.
+    }
+    clear WF.
+    iDestruct "AUTH" as "[AUTH I]".
+    iPoseProof (big_sepM_delete _ _ _ _ Hip with "SAT") as "[[[H1 H2]|H1] SAT]".
+    2: { iCombine "EN H1" as "F". iPoseProof (OwnM_valid with "F") as "%WF".
+         unfold URA.wf, URA.add in WF. unseal "ra". ss. des_ifs. set_solver.
+    }
+    iFrame. unfold wsat. iExists I. iFrame. unfold inv_satall.
+    iApply (big_sepM_delete _ _ _ _ Hip). iFrame.
+  Qed.
 
   Lemma wsat_inv_close i p :
     inv i p ∗ wsat ∗ prop p ∗ OwnD {[i]} ⊢ |==> wsat ∗ OwnE {[i]}.
-  Admitted.
+  Proof.
+    iIntros "(I & [% [AUTH SAT]] & P & DIS)". iModIntro.
+    unfold inv, inv_auth, inv_satall.
+    iCombine "AUTH I" as "AUTH".
+    iPoseProof (OwnM_valid with "AUTH") as "%WF".
+    assert (Hip : I !! i = Some p).
+    { apply Auth.auth_included in WF. rename WF into EXTENDS.
+      apply pw_extends in EXTENDS. specialize (EXTENDS i).
+      unfold maps_to_res in EXTENDS. des_ifs. clear e.
+      rr in EXTENDS. des. unfold URA.add in EXTENDS; unseal "ra".
+      destruct (I !! i) eqn: E.
+      - destruct ctx; ss; des_ifs.
+      - destruct ctx; ss; des_ifs.
+    }
+    clear WF.
+    iDestruct "AUTH" as "[AUTH I]".
+    iPoseProof (big_sepM_delete _ _ _ _ Hip with "SAT") as "[[[H1 H2]|H1] SAT]".
+    { iCombine "DIS H2" as "F". iPoseProof (OwnM_valid with "F") as "%WF".
+      unfold URA.wf, URA.add in WF. unseal "ra". ss. des_ifs. set_solver.
+    }
+    iFrame. unfold wsat. iExists I. iFrame. unfold inv_satall.
+    iApply (big_sepM_delete _ _ _ _ Hip). iFrame. iLeft. iFrame.
+  Qed.
 
 End WORLD_SATISFACTION.
 
